src/Term.v
@@ -10,18 +10,18 @@ Import List.ListNotations.
 
 Set Nested Proofs Allowed.
 
-Lemma wf_lseq_pieces: forall r lr t1 t2,
-    well_formed (alseq r lr t1 t2) ->
-    well_formed t1 /\ well_formed t2.
+Lemma wf_lseq_pieces: forall r t1 t2,
+    well_formed_r (alseq r t1 t2) ->
+    well_formed_r t1 /\ well_formed_r t2.
 Proof.
   intros.
   inversion H.
   tauto.
 Defined.
 
-Lemma wf_at_pieces: forall t r lr locs p q m,
-    well_formed (aatt locs r lr p q m t) ->
-    well_formed t.
+Lemma wf_at_pieces: forall t r p q,
+    well_formed_r (aatt r p q t) ->
+    well_formed_r t.
 Proof.
   intros.
   inversion H.
@@ -50,10 +50,10 @@ Defined.
 
 Ltac do_wf_pieces :=
   match goal with
-  | [H: well_formed (alseq _ _ _ _) |- _] =>
+  | [H: well_formed_r (alseq _ _ _) |- _] =>
     (edestruct wf_lseq_pieces; eauto)
-  | [H: well_formed (aatt _ _ _ _ _ ?t) |- _] =>   
-    assert (well_formed t)
+  | [H: well_formed_r (aatt _ _ _ ?t) |- _] =>   
+    assert (well_formed_r t)
       by (eapply wf_at_pieces; eauto)
   (*| [H: well_formed (abseq _ _ _ _ _) |- _] =>
     (edestruct wf_bseq_pieces; eauto)
@@ -73,7 +73,7 @@ Defined.
 
 Lemma well_formed_range:
   forall t,
-    well_formed t ->
+    well_formed_r t ->
     snd (range t) = fst (range t) + esize t.
 Proof.
   induction t;
@@ -87,13 +87,15 @@ Proof.
     econstructor; eauto. *)
 Defined.
 
+(*
 Lemma well_formed_lrange:
   forall t,
-    well_formed t ->
+    well_formed_r t ->
     length (lrange t) >= anss t.
 Proof.
   induction t; intros H;
     try (simpl; inv H; simpl; repeat concludes; lia).
+*)
 
 Lemma esize_nonempty: forall t, esize t > 0.
 Proof.
@@ -104,7 +106,7 @@ Proof.
 Defined.
 
 Lemma wf_mono: forall t,
-    well_formed t ->
+    well_formed_r t ->
     snd (range t) > fst (range t).
 Proof.
   intros.
@@ -114,12 +116,15 @@ Proof.
   eauto.
 Defined.
 
+Check anno.
+
 Ltac do_mono :=
   (* let asdff := eapply anno_mono; eauto in *)
   match goal with
-  | [H: anno _ ?x _ _ = Some (?y,(_,_)) |- _] => assert_new_proof_by (y > x) ltac:(eapply anno_mono; eauto)
+  | [H: anno _ ?x _ _ = (?y,_) |- _] => assert_new_proof_by (y > x) ltac:(eapply anno_mono; eauto)
   end.
 
+(*
 Lemma asp_lrange_irrel: forall a i l l2 a0 a1 n n' p p' m m' m'' m''',
     anno (asp a) i l m p = Some (n, (m',a0)) ->
     anno (asp a) i l2 m'' p' = Some (n',(m''',a1)) ->
@@ -128,6 +133,7 @@ Proof.
   intros.
   destruct a; ff.
 Defined.
+*)
 
 (*
 Ltac list_facts :=
@@ -154,6 +160,8 @@ Ltac wf_hammer :=
   eauto;
   tauto.
 
+
+(*
 Lemma nodup_lrange: forall t i ls n a p m m',
     NoDup ls ->
     anno t i ls m p = Some (n, (m',a)) ->
@@ -177,7 +185,7 @@ Lemma anno_well_formed:
     length ls = nss t ->
     NoDup ls ->
     anno t i ls m p = Some (j, (m',t')) ->
-    well_formed t'.
+    well_formed_r t'.
 Proof.
   intros.
   generalizeEverythingElse t.
@@ -443,14 +451,15 @@ Proof.
   eassumption.
   eassumption.
 Defined.
+*)
 
 (** Eval for annotated terms. *)
 
 Fixpoint aeval t p e :=
   match t with
-  | aasp _ _ x => eval (asp x) p e
-  | aatt _ _ _ _ q _ x => aeval x q e
-  | alseq _ _ t1 t2 => aeval t2 p (aeval t1 p e)
+  | aasp _ x => eval (asp x) p e
+  | aatt _ _ q x => aeval x q e
+  | alseq _ t1 t2 => aeval t2 p (aeval t1 p e)
   (*| abseq _ _ s t1 t2 => ss (aeval t1 p ((splitEv_T (fst s)) e))
                          (aeval t2 p ((splitEv_T (snd s)) e)) 
   | abpar _ _ _ s t1 t2 => pp (aeval t1 p ((splitEv_T (fst s)) e))
@@ -476,41 +485,41 @@ Defined.
 
 Inductive events: AnnoTerm -> Plc -> Ev -> Prop :=
 | evtscpy:
-    forall r lr i p,
+    forall r i p,
       fst r = i ->
-      events (aasp r lr CPY) p (copy i p)
+      events (aasp r CPY) p (copy i p)
 | evtsusm:
-    forall i id args r lr p,
+    forall i id args r p,
       fst r = i ->
-      events (aasp r lr (ASPC id args)) p (umeas i p id args)
+      events (aasp r (ASPC id args)) p (umeas i p id args)
 | evtssig:
-    forall r lr i p,
+    forall r i p,
       fst r = i ->
-      events (aasp r lr SIG) p (sign i p) 
+      events (aasp r SIG) p (sign i p) 
 | evtshsh:
-    forall r lr i p,
+    forall r i p,
       fst r = i ->
-      events (aasp r lr HSH) p (hash i p)
+      events (aasp r HSH) p (hash i p)
 | evtsattreq:
-    forall r lr q t i p p' req_loc rpy_loc m,
+    forall r q t i p p',
       fst r = i ->
-      events (aatt r lr (req_loc, rpy_loc) p' q m t) p (req i req_loc p q (*(unanno t)*))
+      events (aatt r p' q t) p (req i p q (*(unanno t)*))
 | evtsatt:
-    forall r lr q t ev p p' locs m,
+    forall r q t ev p p',
       events t q ev ->
-      events (aatt r lr locs p' q m t) p ev
+      events (aatt r p' q t) p ev
 | evtsattrpy:
-    forall r lr q t i p p' req_loc rpy_loc m,
+    forall r q t i p p',
       snd r = S i ->
-      events (aatt r lr (req_loc, rpy_loc) p' q m t) p (rpy i rpy_loc p q)
+      events (aatt r p' q t) p (rpy i p q)
 | evtslseql:
-    forall r lr t1 t2 ev p,
+    forall r t1 t2 ev p,
       events t1 p ev ->
-      events (alseq r lr t1 t2) p ev
+      events (alseq r t1 t2) p ev
 | evtslseqr:
-    forall r lr t1 t2 ev p,
+    forall r t1 t2 ev p,
       events t2 p ev ->
-      events (alseq r lr t1 t2) p ev
+      events (alseq r t1 t2) p ev
              (*
 | evtsbseqsplit:
     forall r lr i s t1 t2 p,
@@ -648,10 +657,12 @@ Ltac dest_range :=
   | [H: (nat * nat) |- _] => destruct H
   end.
 
+(*
 Ltac dest_lrange :=
   match goal with
   | [H: LocRange |- _] => destruct H
   end.
+*)
 
 Ltac do_lin_range :=
   match goal with
@@ -687,12 +698,14 @@ Lemma range_lt:
 Proof.
 Admitted.
 
+(*
 Lemma wf_implies_wfr:
   forall x,
     well_formed x ->
     well_formed_r x.
 Proof.
 Admitted.
+*)
 
   
 
@@ -708,7 +721,8 @@ Proof.
       (*destruct r as [j k];*) simpl in *; lia.
 
   -
-    destruct locs.
+    (*
+    destruct locs. *)
     eapply at_range in H2; eauto.
     repeat destruct_disjunct; subst.
     +
