src/CVM_Instr_Alt4.v
@@ -1,0 +1,2841 @@
+Require Import Term_Defs ConcreteEvidence.
+
+Require Import Maps.
+Require Import EqClass.
+
+Require Import List.
+Import ListNotations.
+
+(*
+Require Import RecordSet.
+Import RecordSetNotations.
+*)
+
+Inductive Prim_Instr: Set :=
+| copy: Prim_Instr
+| umeas: ASP_ID -> list Arg -> Prim_Instr
+| sign: Prim_Instr
+| hash: Prim_Instr.
+
+Inductive AnnoInstr: Set :=
+| aprimInstr: nat -> Prim_Instr -> AnnoInstr
+| aReq: nat -> nat -> VM_ID -> AnnoInstr
+| aseq: AnnoInstr -> AnnoInstr -> AnnoInstr.
+
+Definition asp_instr (a:ASP) : Prim_Instr :=
+  match a with
+  | CPY => copy
+  | ASPC i args => umeas i args
+  | SIG => sign
+  | HSH => hash
+  end.
+
+Fixpoint instr_compiler (t:AnnoTerm) : AnnoInstr :=
+  match t with
+  | aasp r a => aprimInstr (fst r) (asp_instr a)
+  | aatt (i,j) p q _ =>
+    (aReq i (Nat.pred j) q)
+  | alseq _ t1 t2 => aseq (instr_compiler t1) (instr_compiler t2)
+  end.
+    
+Definition ev_asp_instr (x:nat) (pi:Prim_Instr) (e:EvidenceC) : EvidenceC :=
+  match pi with
+  | copy => e
+  | umeas asp_id _ => (uuc asp_id x e)
+  | sign => (ggc x e)
+  | hash => (hhc x e)
+  end.
+
+Definition tr_asp_instr (x:nat) (p:Plc) (pi:Prim_Instr) :=
+  match pi with
+  | copy => Term_Defs.copy x p
+  | umeas asp_id args => (Term_Defs.umeas x p asp_id args)
+  | sign => Term_Defs.sign x p
+  | hash => Term_Defs.hash x p
+  end.
+
+
+Inductive InstrSt: Set :=
+| istop: Plc -> EvidenceC -> InstrSt
+| iconf: AnnoInstr -> Plc -> EvidenceC -> InstrSt
+| iWaitReq: VM_ID -> VM_ID -> AnnoInstr -> InstrSt
+| iDoRem: InstrSt -> VM_ID -> InstrSt
+| irpyWait: nat -> VM_ID -> VM_ID -> InstrSt
+| ils: InstrSt -> AnnoInstr -> InstrSt.
+
+(*
+Inductive AnnoInstr: Set :=
+| aprimInstr: nat -> Prim_Instr -> AnnoInstr
+| aReq: nat -> nat -> VM_ID -> VM_ID -> AnnoInstr
+| aseq: AnnoInstr -> AnnoInstr -> AnnoInstr.
+*)
+
+Inductive hLoc : Set :=
+| Empty : hLoc
+| Full: (VM_ID * EvidenceC) -> hLoc.
+    
+Definition heap := hLoc.
+
+Inductive Instr_step: InstrSt -> heap -> option Ev -> InstrSt -> heap -> Prop :=
+| primStep: forall x pi p e h,
+    Instr_step (iconf (aprimInstr x pi) p e) h
+               (Some (tr_asp_instr x p pi))
+               (istop p (ev_asp_instr x pi e)) h
+| atReqStep: forall i p q e h j,
+    Instr_step (iconf (aReq i j q) p e) h
+               (Some (req i p q))
+               (irpyWait j p q) (Full (q,e))
+| atRpyStep: forall j p q e,
+    Instr_step (irpyWait j p q) (Full (p,e))
+               (Some (rpy j p q))
+               (istop p e) Empty
+| atWaitReq: forall p q ai e,
+    Instr_step (iWaitReq p q ai) (Full (q,e))
+               None
+               (iDoRem (iconf ai q e) p) Empty
+| atDoRemStep: forall iSt iSt' h h' ev them,
+    Instr_step iSt h ev iSt' h' ->
+    Instr_step (iDoRem iSt them) h ev (iDoRem iSt' them) h'
+| atDoRemStop: forall p e them h,
+    Instr_step (iDoRem (istop p e) them) h
+               None
+               (istop p e) (Full (them,e))
+| seqStart: forall x y p e h,
+    Instr_step (iconf (aseq x y) p e) h
+               None
+               (ils (iconf x p e) y) h
+| seqStep: forall st0 st1 ev x h h',
+    Instr_step st0 h ev st1 h' ->
+    Instr_step (ils st0 x) h ev (ils st1 x) h'
+| seqStop: forall y p e h,
+    Instr_step (ils (istop p e) y) h None (iconf y p e) h.
+Hint Constructors Instr_step : core.
+
+Require Import Coq.Arith.PeanoNat.
+
+
+Definition add_server_at (fromPl:VM_ID) (toPl:VM_ID) (t:AnnoTerm)
+           (s:MapC VM_ID InstrSt) : MapC VM_ID InstrSt :=
+  let newServerSt := (iWaitReq fromPl toPl (instr_compiler t)) in
+  map_set s toPl newServerSt.  (* TODO:  use map replace instead of set? *)
+    
+Fixpoint copland_compliment (t:AnnoTerm) (s:MapC VM_ID InstrSt): MapC VM_ID InstrSt :=
+  match t with
+  | aasp r a => s
+                   
+  | aatt (i,j) p q t' =>
+    let s' := add_server_at p q t' s in
+    copland_compliment t' s'
+                 
+  | alseq _ t1 t2 =>
+    let s1 := copland_compliment t1 s in
+    copland_compliment t2 s1
+  end.
+
+(* Indicates all servers bound in the map are in a "stop" state *)
+Definition servers_done (servs:MapC VM_ID InstrSt) : Prop :=
+  forall p s,
+    bound_to servs p s ->
+    exists e, s = istop p e.
+
+Require Import Coq.Arith.EqNat.
+
+Open Scope nat_scope.
+
+Definition orchestrate_servers (t:AnnoTerm) (mainPl:Plc) : (MapC VM_ID InstrSt) :=
+  copland_compliment t [].
+
+Definition setup_main_code (t:AnnoTerm) (p:Plc) (e:EvidenceC) : InstrSt :=
+  iconf (instr_compiler t) p e.
+
+Definition WorldTerm := MapC VM_ID InstrSt.
+
+Definition build_world_term_anno (t:AnnoTerm) (p:Plc) (e:EvidenceC) : WorldTerm :=
+  let main := setup_main_code t p e in
+  let servers := orchestrate_servers t p in
+  map_set servers 0 main.
+
+Require Import Place_Facts.
+
+Definition fromSome{A:Type} (default:A) (o:option A) : A :=
+  match o with
+  | Some v => v
+  | None => default
+  end.
+
+
+(*
+Definition build_world_term (t:Term) (p:Plc) (e:EvidenceC):
+  WorldTerm :=
+  let term := fromSome (flatten_term t (flatten_places t)) in
+  build_world_term_anno (annotated t p) p e.
+*)
+
+Inductive platStep : WorldTerm -> heap -> option Ev ->
+                     WorldTerm -> heap -> Type :=
+| platStepServer: forall i i' ev h h' p servs,
+    bound_to servs p i ->
+    Instr_step i h ev i' h' ->
+    platStep servs
+             h ev
+             (map_replace servs p i')
+             h'.
+
+Inductive lstar_world: WorldTerm -> heap -> list Ev -> WorldTerm -> heap -> Prop :=
+| lstar_refl: forall w h, lstar_world w h [] w h
+| lstar_tran: forall e tr wt wt' wt'' h h' h'',
+    platStep wt h (Some e) wt' h' ->
+    lstar_world wt' h' tr wt'' h'' ->
+    lstar_world wt h (e :: tr) wt'' h''
+| lstar_silent_tran: forall wt wt' wt'' h h' h'' tr,
+    platStep wt h None wt' h' ->
+    lstar_world wt' h' tr wt'' h'' ->
+    lstar_world wt h tr wt'' h''.
+Hint Resolve lstar_refl : core.
+
+Require Import LTS.
+
+Check annotated.
+
+Definition get_flattened_term (t:Term) : Term :=
+  fromSome (asp CPY) (flatten_term t (flatten_places t)).
+
+Require Import Coq.Program.Tactics.
+Require Import Auto.
+
+
+(* (* TODO:  I don't think this holds ... *)
+Lemma unique_reqs: forall t p p',
+  term_places_r t p ->
+  term_places_r t p' ->
+  p <> p'.
+Proof.
+Admitted.
+ *)
+
+Definition reqs_mono_starting_at (t:Term) (n:nat) : Prop.
+Admitted.
+
+Definition reqs_mono_starting_at_anno (t:AnnoTerm) (n:nat) : Prop.
+Admitted.
+
+Lemma mono_if_flattened: forall t,
+    reqs_mono_starting_at (get_flattened_term t) 1.
+Proof.
+Admitted.
+
+Lemma reqs_mono_anno: forall t,
+    reqs_mono_starting_at t 1 ->
+    reqs_mono_starting_at_anno (annotated t 0) 0.
+Proof.
+Admitted.
+
+
+(*
+(build_world_term_anno (annotated (get_flattened_term t') p) p e)
+*)
+Lemma world_refines_lts_event_ordering:
+  forall t p e h' tr servs',
+    reqs_mono_starting_at_anno t 0 ->
+    lstar_world (build_world_term_anno t p e)  Empty tr servs'  h' ->
+    servers_done servs' ->
+    LTS.lstar (conf t p mt) tr (stop p (aeval t p mt)).
+Proof.
+  intros.
+
+  (*
+  assert (exists x, flatten_term t' (flatten_places t') = Some x).
+  eapply flatten_some; eauto.
+  destruct_conjs.
+  unfold get_flattened_term in *.
+  unfold fromSome in *.
+  rewrite H2 in *.
+  assert (well_formed_r (annotated H1 p)). admit.
+*)
+
+  generalizeEverythingElse t.
+  induction t; intros.
+  -
+    df.
+    unfold build_world_term_anno in *.
+    unfold orchestrate_servers in *.
+    unfold copland_compliment in *.
+    unfold setup_main_code in *.
+    df.
+    unfold map_set in *.
+
+    destruct a.
+    +
+      invc H0.
+      ++
+        unfold servers_done in *.
+
+        pose (H1 0 (iconf (aprimInstr (fst r) (asp_instr CPY)) p e)).
+        edestruct e0.
+        econstructor.
+        df.
+        tauto.
+        solve_by_inversion.
+      ++
+        admit.
+
+      ++
+        admit.
+    +
+      admit.
+    +
+      admit.
+    +
+      admit.
+  -
+
+Abort.
+
+
+
+
+HERE
+
+  
+ 
+
+
+
+
+
+
+
+
+
+
+
+
+
+
+
+
+
+
+
+
+
+Inductive is_waiting: Plc -> VM_ID -> InstrSt -> Prop :=
+| immedWaitReq: forall i p q vmid,
+    is_waiting q vmid (iWaitReq p (q,vmid) i).
+
+(* | willDo: forall fromPair iSt,
+    (* TODO: do we need to recurse on iSt here? *)
+    will_respond fromPair (iDoRem iSt fromPair). *)
+                           
+
+
+
+
+Inductive ws_instr: AnnoInstr -> (Plc*VM_ID) -> MapC (Plc*VM_ID) InstrSt -> Prop :=
+| wsi_prim: forall i p pr m,
+    ws_instr (aprimInstr i p) pr m
+| wsi_req: forall i j req_loc rpy_loc p q vmi m iSt,
+    bound_to m (q,vmi) iSt ->
+    is_waiting q vmi iSt ->
+    p <> q -> (* TODO: is this necessary? *) 
+    ws_instr (aReq i j req_loc rpy_loc p (q,vmi)) (p,vmi) m
+| wsi_seq: forall a1 a2 pr m,
+    ws_instr a1 pr m ->
+    ws_instr a2 pr m ->
+    ws_instr (aseq a1 a2) pr m.
+
+(*
+Inductive will_request_instr: (Plc*VM_ID) -> AnnoInstr -> Prop :=
+| wreq: forall p q i j req_loc rpy_loc vmi,
+    will_request_instr (q,vmi) (aReq i j req_loc rpy_loc p (q,vmi))
+| wseql: forall pr a1 a2,
+    will_request_instr pr a1 ->
+    will_request_instr pr (aseq a1 a2)
+| wseqr: forall pr a1 a2,
+    will_request_instr pr a2 ->
+    will_request_instr pr (aseq a1 a2).
+
+
+Inductive will_request: (Plc*VM_ID) -> InstrSt -> Prop :=
+| wrconf: forall i p e pr,
+    will_request_instr pr i ->
+    will_request pr (iconf i p e)
+| will_request 
+ *)
+
+Inductive will_request_instr:  (Plc*VM_ID) -> AnnoInstr -> MapC (Plc*VM_ID) InstrSt -> Prop :=
+| wriReq:
+    forall q vmi i j x y p m,
+      will_request_instr (q,vmi) (aReq i j x y p (q,vmi)) m
+| wrseql: forall q q' a1 m a2 vmi,
+    will_request_instr (q',vmi) a1 m ->
+    q <> q' ->
+    (forall iSt, bound_to m (q',vmi) iSt -> is_waiting q' vmi iSt) ->
+    will_request_instr (q,vmi) (aseq a1 a2) m.
+
+
+Inductive will_request: (Plc*VM_ID) -> InstrSt -> MapC (Plc*VM_ID) InstrSt -> Prop :=
+| will_request (q,vmi) (
+
+
+Inductive ws_world: MapC (Plc*VM_ID) InstrSt (*-> heap*) -> Prop :=
+| wsw_stop: forall m,
+    servers_done m ->
+    ws_world  m
+| wsw_conf: forall i m vmi e p,
+    bound_to m (p,vmi) (iconf i p e) ->
+    ws_instr i (p,vmi) m -> 
+    ws_world m
+| wsw_waitReq: forall p q vmi ai iSt m,
+    bound_to m (q,vmi) (iWaitReq p (q,vmi) ai) ->
+    bound_to m (p,vmi) iSt ->
+    p <> q ->
+    will_request (q,vmi) iSt m -> 
+    ws_world m.
+
+
+
+| wsw_rpyWait: forall m p q iSt j rpy_loc,
+    bound_to m q iSt ->
+    will_respond p iSt ->
+    ws_world (irpyWait j rpy_loc p q) m
+| wsw_ls: forall m m' iSt ai,
+    ws_world iSt m ->
+    advance_servers_ist iSt m m' ->
+    ws_instr ai m' -> (* TODO:  pl (iSt)? *)
+    servers_done m' ->
+    ws_world (ils iSt ai) m.
+
+Set Nested Proofs Allowed.
+
+
+Lemma well_structured_world_init: forall t p e,
+    well_formed t ->
+    ws_world (iconf (instr_compiler t) p e) (copland_compliment t []).
+Proof.
+  intros.
+  generalizeEverythingElse t.
+  induction t; intros.
+  -
+    destruct a;
+      df;
+      repeat econstructor.
+  -
+    df.
+    subst.
+    unfold map_set in *.
+    df.
+    apply wsw_conf.
+    
+    econstructor.
+    econstructor.
+    +
+      unfold map_set in *.
+      unfold map_get in *.
+
+    rewrite Nat.eqb_refl in *.
+    eauto.
+    +
+      
+    econstructor.
+  -
+    do_wf_pieces.
+    econstructor.
+
+    assert (ws_world (iconf (instr_compiler t1) p e) (copland_compliment t1 [])) by eauto.
+
+    assert (ws_world (iconf (instr_compiler t2) p e) (copland_compliment t2 [])) by eauto.
+
+    eapply compliment_alseq_skip'.
+
+    repeat find_inversion.
+
+    invc H2.
+    invc H3.
+    df.
+    eapply compliment_focus; eauto.
+
+    df.
+    eapply advance_assoc; eauto.
+    solve_by_inversion.
+Defined.
+*)
+
+
+
+
+
+
+
+
+
+Lemma platStep_ws: forall wt h ev wt' h',
+  well_structured_world wt ->
+  platStep wt h ev wt' h' ->
+  well_structured_world wt'.
+Proof.
+  intros.
+  destruct wt.
+  destruct wt'.
+
+  invc X.
+  admit.
+  admit.
+  admit.
+
+  generalizeEverythingElse i.
+  induction i; intros.
+  -
+    invc H.
+    invc X; try solve_by_inversion.
+    econstructor.
+    econstructor.
+    econstructor.
+  -
+    invc H.
+    invc X.
+    +
+      invc H7.
+      ++
+        econstructor.
+      ++
+        invc H4.
+        econstructor.
+        eassumption.
+        eassumption.
+      ++
+        invc H4.
+        
+        econstructor.
+        +++
+          econstructor.
+          eassumption.
+        +++
+          eapply advance_ist_iff; eauto.
+        +++
+          eassumption.
+        +++
+          eassumption.
+    +
+      econstructor.
+      admit.
+    +
+      econstructor.
+      admit.
+    +
+      econstructor.
+      
+      
+          
+          
+    
+        
+        
+          
+          
+          
+        
+        invc H4.
+        apply H7.
+    
+
+
+
+
+  
+  generalizeEverythingElse H.
+  induction H; intros.
+  -
+    invc X; try solve_by_inversion.
+    econstructor.
+    econstructor.
+    econstructor.
+    
+  -
+    invc X; try solve_by_inversion.
+    +
+      invc H7; try solve_by_inversion.
+      ++
+        econstructor.
+      ++
+        invc H.
+        econstructor.
+        eassumption.
+        eassumption.
+      ++
+        invc H.
+        econstructor.
+        econstructor.
+        eassumption.
+
+
+
+        eapply advance_ist_iff; eauto.
+
+        eassumption.
+        eassumption.
+        
+        
+    +
+      invc H7.
+      econstructor.
+      admit.
+    +
+      econstructor.
+      admit.
+    +
+      econstructor.
+      
+      
+    
+    
+    inversion H.
+    inversion X; try solve_by_inversion.
+    econstructor.
+    rewrite H10.
+    subst.
+    invc X
+
+  
+
+
+(*
+| platStepOneDone: forall i h h' ev p e,
+    Instr_step i h ev (istop p e) h' ->
+    platStep_l (onePlat i) h ev (donePlat p e) h'
+| platStepPar_l: forall wt1 wt1' wt2 h h' ev,
+    platStep_l wt1 h ev wt1' h' ->
+    platStep_l (parPlats wt1 wt2) h ev (parPlats wt1' wt2) h'
+| platStepPar_r: forall wt1 wt2 wt2' h h' ev,
+    platStep_l wt2 h ev wt2' h' ->
+    platStep_l (parPlats wt1 wt2) h ev (parPlats wt1 wt2') h'
+| platStepDone: forall p q h e e',
+    platStep_l (parPlats (donePlat p e) (donePlat q e')) h None (donePlat p e) h.
+*)
+
+(*
+Inductive platStep : InstrSt -> configs -> heap -> option Ev ->
+                     InstrSt -> configs -> heap -> Type :=
+| mainStep: forall i i' ev w h h',
+    Instr_step i h ev i' h' ->
+    platStep i w h ev i' w h'
+| worldStep: forall p w wi wi' ev i h h',
+    bound_to w p wi ->
+    Instr_step wi h ev wi' h' ->
+    platStep i w h ev i (map_set w p wi') h'.
+*)
+
+(*
+Definition world_config := (InstrSt*configs*heap)%type.
+ *)
+
+
+
+(*
+
+Inductive lstar_world: world_config -> list Ev -> world_config -> Prop :=
+| lstar_refl: forall w, lstar_world w [] w
+| lstar_tran: forall e tr i i' c c' h h' st2,
+    platStep i c h (Some e) i' c' h' ->
+    lstar_world (i',c',h') tr st2 ->
+    lstar_world (i,c,h) (e :: tr) st2
+| lstar_silent_tran: forall tr i i' c c' h h' st2,
+    platStep i c h None i' c' h' -> lstar_world (i',c',h') tr st2 ->
+    lstar_world (i,c,h) tr st2.
+Hint Resolve lstar_refl : core.
+ *)
+
+Require Import LTS Auto.
+
+Definition asp1 := asp (ASPC 1 []).
+Definition asp2 := asp (ASPC 2 []).
+
+Definition ex1_term :=
+  lseq (att 1 asp1) asp2. (*(att 1 asp2)*)
+  (*att 1 asp1 *) 
+
+Definition ex1_term_annotated :=
+  snd (anno' ex1_term 0 [42;43] 2 ).
+
+(*
+Definition ex1_heap := [(42,Empty);(43,Empty)].
+Check ex1_heap.
+*)
+
+Compute ex1_term_annotated.
+
+Compute (orchestrate_l_servers ex1_term_annotated).
+Compute (build_world_term ex1_term_annotated 2 mtc).
+
+Compute (copland_compliment_l (snd (anno' (att 1 asp1) 0 [42;43] 2)) []).
+
+Compute (copland_compliment_l ex1_term_annotated []).
+
+Compute (build_world_term ex1_term_annotated 2 mtc).
+
+(*
+Ltac inv_lstar :=
+  match goal with
+  (*|[H: locContains (?C) _ _  |- _ ] => invc H
+  | [H: locEmpty (?C) (*(put_heap _ _ _)*) _  |- _ ] => invc H *)
+  | [H: Instr_step (?C _) _ _ _ _  |- _ ] => invc H
+                                                (*
+  | [H: platStep
+          (onePlat (?C _)) _ _ _ _ |- _ ] => invc H
+  | [H: platStep
+          (parPlats (?C _) _) _ _ _ _ |- _ ] => invc H
+  | [H: lstar_world
+          (parPlats (?C _) _) _ _ _ _ |- _] => invc H
+*)
+  end;
+  df;
+  try solve_by_inversion.
+*)
+
+
+Set Nested Proofs Allowed.
+
+  Ltac do_eqb_reflect :=
+    let H_eq := fresh in
+    match goal with
+    | [H: eqb ?p ?n = true |- _] =>
+      assert_new_proof_as_by
+        (p = n)
+        ltac:(eapply eqb_leibniz; apply H)
+               H_eq;
+      clear H
+    end;
+    rewrite H_eq in *;
+    clear H_eq.
+
+  Ltac bound_facts :=
+    match goal with
+    | [H: bound_to [] _ _ |- _] =>
+      invc H; unfold map_get in *; solve_by_inversion
+    | [H: bound_to _ _ _ |- _] =>
+      invc H
+    end;
+    unfold map_get in *;
+    break_if; try solve_by_inversion;
+    do_eqb_reflect;
+    unfold map_replace in *;
+    unfold map_remove in *;
+    subst;
+    df;
+    unfold map_set in *;
+    repeat rewrite Nat.eqb_refl in *;
+    df.
+
+
+  
+  (*
+  Ltac bound_facts :=
+    match goal with
+    | [H: bound_to _ _ _ |- _] =>
+      invc H
+    end;
+    unfold map_get in *;
+    break_if; try solve_by_inversion;
+    do_eqb_reflect;
+    unfold map_replace in *;
+    unfold map_remove in *;
+    subst;
+    df;
+    unfold map_set in *;
+    df.
+*)
+
+  Ltac inv_lstar :=
+  match goal with
+  (*|[H: locContains (?C) _ _  |- _ ] => invc H
+  | [H: locEmpty (?C) (*(put_heap _ _ _)*) _  |- _ ] => invc H *)
+  | [H: Instr_step (?C _) _ _ _ _  |- _ ] => invc H
+
+  | [H:
+       platStep
+        (worldTermC (?C _) (*(iconf _ _ _)*) _)
+        _ _ _ _ |- _] => invc H
+  (*
+  | [H: platStep
+          (parPlats (?C _) _) _ _ _ _ |- _ ] => invc H
+*)
+  | [H: lstar_world
+          (worldTermC (?C _) _) _ _ _ _ |- _] => invc H
+  end;
+  (*try unfold wrap_server_config in *; *)
+  df;
+  try solve_by_inversion.
+
+Ltac unfold_world_defs :=
+  unfold build_world_term in *;
+  unfold orchestrate_l_servers in *;
+  unfold setup_main_code in *;
+  df;
+  unfold wrap_server_config in *;
+  df.
+
+Definition ex1_heap : heap := Empty. (* option (Plc*EvidenceC) := None. *)
+
+Definition ex1_world : WorldTerm := (build_world_term ex1_term_annotated 2 mtc).
+
+(*
+Lemma world_refines_lts_event_ordering_ex1:
+  forall (*t p e*) e' (*h*) h' tr servs' (*et*) (*(wt:WorldTerm)*) ,
+    (*well_formed t -> *)
+    (* let wt := build_world_term t p e in (*(InstrSt*configs)*) *)
+    
+    lstar_world ex1_world ex1_heap tr (worldTermC (istop 2 e') servs')  h' ->
+    LTS.lstar (conf ex1_term_annotated 2 mt) tr (stop 2 (aeval ex1_term_annotated 2 mt)).
+Proof.
+  intros.
+  unfold ex1_world in *.
+  unfold ex1_term_annotated in *.
+  unfold_world_defs.
+
+  (*
+  unfold build_world_term in *.
+  unfold orchestrate_l_servers in *.
+  unfold setup_main_code in *.
+  (*
+  unfold build_world_term' in *.
+  unfold build_world_term'' in *. *)
+  unfold ex1_term_annotated in *.
+  df.
+  unfold wrap_server_config in *.
+  df.
+  (*
+  unfold combineInstrSt in *. *)
+  unfold ex1_heap in *.
+
+  (*
+  unfold wrap_server_config in *. *)
+  (*unfold build_one' in *. *)
+
+  df.
+*)
+
+  repeat (inv_lstar; try bound_facts).
+
+
+  -
+  eapply lstar_silent_tran.
+  econstructor.
+
+  eapply lstar_tran.
+  econstructor.
+
+  econstructor.
+
+  eapply lstar_tran.
+  econstructor.
+  eapply stattstep.
+  econstructor.
+
+  eapply lstar_tran.
+  econstructor.
+  eapply stattstop.
+
+  eapply lstar_silent_tran.
+  eapply stlseqstop.
+
+  eapply lstar_tran.
+  econstructor.
+  econstructor.
+  -
+      eapply lstar_silent_tran.
+  econstructor.
+
+  eapply lstar_tran.
+  econstructor.
+
+  econstructor.
+
+  eapply lstar_tran.
+  econstructor.
+  eapply stattstep.
+  econstructor.
+
+  eapply lstar_tran.
+  econstructor.
+  eapply stattstop.
+
+  eapply lstar_silent_tran.
+  eapply stlseqstop.
+
+  eapply lstar_tran.
+  econstructor.
+  econstructor.
+  -
+      eapply lstar_silent_tran.
+  econstructor.
+
+  eapply lstar_tran.
+  econstructor.
+
+  econstructor.
+
+  eapply lstar_tran.
+  econstructor.
+  eapply stattstep.
+  econstructor.
+
+  eapply lstar_tran.
+  econstructor.
+  eapply stattstop.
+
+  eapply lstar_silent_tran.
+  eapply stlseqstop.
+
+  eapply lstar_tran.
+  econstructor.
+  econstructor.
+  -
+      eapply lstar_silent_tran.
+  econstructor.
+
+  eapply lstar_tran.
+  econstructor.
+
+  econstructor.
+
+  eapply lstar_tran.
+  econstructor.
+  eapply stattstep.
+  econstructor.
+
+  eapply lstar_tran.
+  econstructor.
+  eapply stattstop.
+
+  eapply lstar_silent_tran.
+  eapply stlseqstop.
+
+  eapply lstar_tran.
+  econstructor.
+  econstructor.
+  -
+      eapply lstar_silent_tran.
+  econstructor.
+
+  eapply lstar_tran.
+  econstructor.
+
+  econstructor.
+
+  eapply lstar_tran.
+  econstructor.
+  eapply stattstep.
+  econstructor.
+
+  eapply lstar_tran.
+  econstructor.
+  eapply stattstop.
+
+  eapply lstar_silent_tran.
+  eapply stlseqstop.
+
+  eapply lstar_tran.
+  econstructor.
+  econstructor.
+  -
+      eapply lstar_silent_tran.
+  econstructor.
+
+  eapply lstar_tran.
+  econstructor.
+
+  econstructor.
+
+  eapply lstar_tran.
+  econstructor.
+  eapply stattstep.
+  econstructor.
+
+  eapply lstar_tran.
+  econstructor.
+  eapply stattstop.
+
+  eapply lstar_silent_tran.
+  eapply stlseqstop.
+
+  eapply lstar_tran.
+  econstructor.
+  econstructor.
+  Defined.
+    
+    
+    
+    
+    
+
+
+  (*
+  econstructor.
+  apply 
+
+  apply stattstep.
+  econstructor.
+  eapply lstar_tran.
+  econstructor.
+
+  eapply stattstep.
+
+  
+  apply stattstop.
+
+  eapply lstar_tran
+
+  
+  econstructor.
+  econstructor.
+  apply stattstop.
+
+  simpl.
+
+  econstructor
+  
+  
+  eapply statt.
+  eapply lstar_tran.
+  eapply stattstep.
+  econstructor.
+  eapply lstar_tran.
+  apply stattstop.
+  apply lstar_refl.
+  
+
+  eapply lstar_tran.
+  eapply statt.
+  eapply lstar_tran.
+  eapply stattstep.
+  econstructor.
+  eapply lstar_tran.
+  apply stattstop.
+  apply lstar_refl.
+
+  eapply lstar_tran.
+  eapply statt.
+  eapply lstar_tran.
+  eapply stattstep.
+  econstructor.
+  eapply lstar_tran.
+  apply stattstop.
+  apply lstar_refl.
+
+  eapply lstar_tran.
+  eapply statt.
+  eapply lstar_tran.
+  eapply stattstep.
+  econstructor.
+  eapply lstar_tran.
+  apply stattstop.
+  apply lstar_refl.
+*)
+
+ *)
+
+(*
+    Ltac bound_facts' :=
+    match goal with
+    | [H: bound_to [] _ _ |- _] =>
+      invc H; unfold map_get in *; solve_by_inversion
+    | [H: bound_to _ _ _ |- _] =>
+      invc H
+    end;
+    unfold map_get in *;
+    break_if; try solve_by_inversion;
+    do_eqb_reflect;
+    unfold map_replace in *;
+    unfold map_remove in *;
+    subst;
+    df;
+    unfold map_set in *;
+    df.
+ *)
+
+
+Lemma combine_lem{A B:Type} `{H : EqClass A} : forall (prs:(list (A*B))),
+    combine (map_dom prs) (map_vals prs) = prs.
+Proof.
+  intros.
+  induction prs.
+  -
+    tauto.
+  -
+    simpl.
+    repeat break_let.
+    subst.
+    simpl.
+    rewrite IHprs.
+    tauto.
+Defined.
+
+Lemma lstar_world_lseq_decomp: forall t1 t2 p e e'' h' servs' tr l r,
+
+    (*
+    lstar_world
+      (worldTermC (iconf (aseq (instr_compiler t1) (instr_compiler t2)) p e)
+                  (combine (map_dom (copland_compliment_l t2 (copland_compliment_l t1 [])))
+                           (map wrap_server_config (copland_compliment_l t2 (copland_compliment_l t1 []))))) Empty tr
+      (worldTermC (istop p e'') servs') h' -> 
+     *)
+
+    well_formed (alseq r l t1 t2) ->
+
+
+    lstar_world
+         (worldTermC (iconf (instr_compiler (alseq r l t1 t2)) p e)
+            (combine (map_dom (copland_compliment_l (alseq r l t1 t2) []))
+               (map wrap_server_config (copland_compliment_l (alseq r l t1 t2) [])))) Empty tr
+         (worldTermC (istop p e'') servs') h' ->
+
+    exists (tr1: list Ev) e_mid servs_mid (*(h_mid:heap)*),
+      lstar_world
+        (worldTermC (iconf (instr_compiler t1) p e)
+                    (combine (map_dom (copland_compliment_l t1 [])) (map wrap_server_config (copland_compliment_l t1 [])))) Empty tr1
+        (worldTermC (istop p e_mid) servs_mid) Empty /\
+      servers_done servs_mid /\
+      exists (tr2: list Ev),
+        lstar_world
+          (worldTermC (iconf (instr_compiler t2) p e_mid)
+                      (combine (map_dom (copland_compliment_l t2 [])) (map wrap_server_config (copland_compliment_l t2 [])))) Empty (*h_mid*) tr2
+          (worldTermC (istop p e'') servs') h' /\
+        servers_done servs' /\
+        tr = tr1 ++ tr2.
+Proof.
+  intros.
+  df.
+  do_wf_pieces.
+  df.
+  repeat eexists.
+  
+  inv_lstar.
+  admit.
+
+Abort.
+
+Lemma evshape_trace_irrel : forall t p et et' et2 et2' tr,
+    lstar (conf t p et)  tr (stop p et') ->
+    lstar (conf t p et2) tr (stop p et2').
+Proof.
+Admitted.
+
+Require Import Coq.Program.Tactics.
+
+Check bound_to.
+
+
+
+(*
+Lemma at_world_decomp :
+  forall t n0 e tr0 n4 n2 st1 servs_res e_res h' h'0 n,
+
+    lstar_world
+      (worldTermC
+         (irpyWait (Init.Nat.pred n2) n4 n0 n0)
+         [(n0, ils st1 (aResp (Nat.pred n2) n))])
+      h'0
+      tr0
+      (worldTermC (istop n0 e_res) servs_res) h' -> 
+    Instr_step (iconf (instr_compiler t) n0 e) Empty None st1 h'0 -> 
+    
+
+    
+    exists tr e' servs' h',
+      lstar_world
+        (worldTermC (iconf (instr_compiler t) n0 e)
+                    (combine (map_dom (copland_compliment_l t [])) (map wrap_server_config (copland_compliment_l t [])))) Empty tr
+        (worldTermC (istop n0 e') servs') h' /\
+      servers_done servs' /\
+      (tr0 = tr ++ [(rpy (Init.Nat.pred n2) n4 n0 n0)]).
+Proof.
+Admitted.
+ *)
+
+Lemma at_world_decomp' : forall t n1 n2 n3 n4 n0 p0 e n tr e' servs' h',
+    lstar_world
+      (worldTermC
+         (iconf (aReq n1 (Init.Nat.pred n2) n3 n4 n0) p0 e)
+         [(n0,
+           (iconf
+              (aseq
+                 (aseq (aWaitReq n1) (instr_compiler t))
+                 (aResp (Nat.pred n2) n)) n0 mtc))])
+      Empty
+      tr
+      (worldTermC (istop p0 e') servs') h' ->
+    lstar_world
+      (worldTermC
+         (iconf (aReq n1 (Init.Nat.pred n2) n3 n4 n0) p0 e)
+         [(n0,
+           (iconf
+              (aseq
+                 (aseq (aWaitReq n1) (instr_compiler t))
+                 (aResp (Nat.pred n2) n)) n0 mtc))])
+      Empty
+      [(req n1 n3 p0 n0)]
+      (worldTermC
+         (irpyWait (Init.Nat.pred n2) n4 n0 p0)
+         [(n0,
+           ils (iconf (instr_compiler t) n0 e)
+               (aResp (Nat.pred n2) n))])
+      Empty /\
+    exists s_ev t_tr,
+      lstar_world
+        (worldTermC
+           (irpyWait (Init.Nat.pred n2) n4 n0 p0)
+           [(n0,
+             ils (iconf (instr_compiler t) n0 e)
+                 (aResp (Nat.pred n2) n))])
+        Empty
+        t_tr
+        (worldTermC
+           (irpyWait (Init.Nat.pred n2) n4 n0 p0)
+           [(n0, (istop n0 s_ev))])
+        (Full (p0,s_ev)) /\
+      tr = [(req n1 n3 p0 n0)] ++ t_tr ++ [(rpy (Init.Nat.pred n2) n4 p0 n0)]. 
+Proof.
+Admitted.
+
+Lemma remote_same: forall n2 n4 n0 p0 e n H4 H3 t,
+    lstar_world
+      (worldTermC
+         (irpyWait (Init.Nat.pred n2) n4 n0 p0)
+         [(n0, ils (iconf (instr_compiler t) n0 e) (aResp (Nat.pred n2) n))])
+      Empty
+      H4
+      (worldTermC
+         (irpyWait (Init.Nat.pred n2) n4 n0 p0)
+         [(n0, istop n0 H3)])
+      (Full (p0, H3)) ->
+    exists servs'' h'',
+      lstar_world
+        (worldTermC
+           (iconf (instr_compiler t) n0 e)
+           (combine (map_dom (copland_compliment_l t [])) (map wrap_server_config (copland_compliment_l t []))))
+        Empty
+        H4
+        (worldTermC (istop n0 H3) servs'') h'' /\
+      servers_done servs''.
+Proof.
+Admitted.
+
+
+Lemma world_refines_lts_event_ordering:
+  forall t p e e' (*h*) h' tr servs' (*et*) (*(wt:WorldTerm)*) ,
+    well_formed t ->
+    (*let wt := build_world_term t p e in (*(InstrSt*configs)*) *)
+    
+    lstar_world (build_world_term t p e) Empty tr (worldTermC (istop p e') servs')  h' ->
+    servers_done servs' ->
+    LTS.lstar (conf t p mt) tr (stop p (aeval t p mt)).
+Proof.
+  intros.
+  unfold_world_defs.
+
+  unfold mapify_server_configs in *.
+  unfold init_configs in *.
+  df.
+  assert (
+      (combine (map_dom (copland_compliment_l t [])) (map_vals (copland_compliment_l t []))) =
+      (copland_compliment_l t [])).
+  {
+    eapply combine_lem; eauto.
+  }
+  repeat rewrite H2 in *; clear H2.
+  (*
+  unfold wrap_server_config in *.
+  unfold map_vals in *.
+  unfold copland_compliment_l in *. 
+   *)
+
+  generalizeEverythingElse t.
+  induction t; intros.
+  -
+    destruct a; df;
+      repeat (inv_lstar; try bound_facts; try (econstructor; econstructor; tauto)).
+  -
+    df.
+    (*
+    unfold wrap_server_config in *. *)
+    df.
+
+    (*
+    assert (
+        exists ev_res, 
+    lstar_world
+      (worldTermC
+         (iconf (aReq n1 (Init.Nat.pred n2) n3 n4 n0) p0 e)
+         [(n0, iconf
+                 (aseq
+                    (aseq (aWaitReq n1) (instr_compiler t))
+                    (aResp (Nat.pred n2) n))
+                 n0
+                 mtc)])
+      Empty
+      tr
+      (worldTermC
+         (istop p0 ev_res)
+         [n0,
+          ils (ils (iconf (instr_compiler t) n0 e)
+
+      
+
+
+
+      
+      (worldTermC (istop p0 e') servs') h')
+*)
+
+
+
+
+
+           (*
+    lstar_world
+      (worldTermC
+         (iconf (aReq n1 (Init.Nat.pred n2) n3 n4 n0) p0 e)
+         [(n0, iconf
+                 (aseq
+                    (aseq (aWaitReq n1) (instr_compiler t))
+                    (aResp (Nat.pred n2) n))
+                 n0
+                 mtc)])
+      Empty
+      tr
+      (worldTermC (istop p0 e') servs') h') *)
+
+
+    subst.
+    unfold wrap_server_config in H0.
+    df.
+
+
+
+
+    edestruct at_world_decomp'.
+    eassumption.
+    destruct_conjs.
+    subst.
+
+
+
+    edestruct remote_same.
+    eassumption.
+    destruct_conjs.
+
+    eapply lstar_transitive.
+
+    eapply lstar_tran.
+    apply statt.
+    econstructor.
+
+    eapply lstar_transitive.
+
+    eapply lstar_strem.
+
+    eapply IHt.
+    invc H.
+    eauto.
+
+
+
+    
+    
+
+    eassumption.
+    eassumption.
+
+    eapply lstar_tran.
+    apply stattstop.
+    econstructor.
+
+    (*
+
+        H5 : lstar_world (worldTermC (irpyWait (Init.Nat.pred n2) n4 n0 p0) [(n0, ils (iconf (instr_compiler t) n0 e) (aResp (Nat.pred n2) n))]) Empty H4
+         (worldTermC (irpyWait (Init.Nat.pred n2) n4 n0 p0) [(n0, istop n0 H3)]) (Full (p0, H3))
+  ============================
+  lstar_world
+    (worldTermC (iconf (instr_compiler t) n0 ?e) (combine (map_dom (copland_compliment_l t [])) (map wrap_server_config (copland_compliment_l t []))))
+    Empty H4 (worldTermC (istop n0 ?e') ?servs') ?h'
+     *)
+    
+
+
+    (*
+
+    
+    eassumption.
+
+    
+
+    
+    eassumption.
+    
+
+    exfalso.
+    eapply at_world_decomp'; eauto.
+
+      
+   
+      
+      
+
+
+
+
+
+
+
+
+
+
+
+
+
+
+
+
+    
+
+    
+
+
+
+
+
+
+    
+    inv_lstar.
+    inv_lstar.
+    inv_lstar.
+
+    unfold wrap_server_config in H2.
+    df.
+
+    
+    inv_lstar.
+    inv_lstar.
+    inv_lstar.
+    inv_lstar.
+
+    Ltac servers_done_contra :=
+      unfold servers_done in *;
+      (*unfold wrap_server_config in *; *)
+      df;
+      let HH := fresh in
+      match goal with
+      | [(*H: servers_done [(?C _)], *)
+            H: context[
+                    bound_to [(?n0, ?s)] _ _ -> _] |- _] =>
+        pose (H n0 s) as HH;
+        forward HH
+      end;
+      econstructor;
+        df;
+        try rewrite Nat.eqb_refl;
+        try tauto;
+        try (concludes; destruct_conjs; bound_facts).
+
+    servers_done_contra.
+    
+(*
+    concludes.
+    destruct_conjs.
+    bound_facts.
+
+
+
+    forward e.
+        
+
+
+    
+    unfold servers_done in *.
+    unfold wrap_server_config in *.
+    df.
+    specialize H1 with (p:=n0) (s:=(iconf (aseq (aseq (aWaitReq n1) (instr_compiler t)) (aResp (Nat.pred n2) n)) n0 mtc)).
+    destruct_conjs.
+
+    forward H1.
+    econstructor.
+    df.
+    Search (_ =? _).
+    rewrite Nat.eqb_refl.
+    tauto.
+    concludes.
+    destruct_conjs.
+    bound_facts.
+ *)
+    
+
+    inv_lstar.
+    bound_facts.
+    inv_lstar.
+    inv_lstar.
+    bound_facts.
+    inv_lstar.
+    inv_lstar.
+    servers_done_contra.
+    inv_lstar.
+    bound_facts.
+    inv_lstar.
+    inv_lstar.
+    bound_facts.
+    inv_lstar.
+    inv_lstar.
+    inv_lstar.
+    servers_done_contra.
+    inv_lstar.
+    bound_facts.
+    inv_lstar.
+
+    fold wrap_server_config in IHt.
+    inv_lstar.
+    inv_lstar.
+    bound_facts.
+    inv_lstar.
+    inv_lstar.  
+    bound_facts.
+    inv_lstar.
+
+    inv_lstar.
+    bound_facts.
+    inv_lstar.
+
+    (*
+    Require Import Coq.Arith.PeanoNat. *)
+
+    destruct (Nat.eq_dec p0 n0).
+    +
+      subst.
+      (*
+      repeat (inv_lstar; try bound_facts; try servers_done_contra; try bound_facts; try servers_done_contra).
+       *)
+      
+      inv_lstar.
+      
+      (* Main thread grabbed evidence *)
+      inv_lstar.
+      inv_lstar.
+      inv_lstar.
+      servers_done_contra.
+      inv_lstar.
+      bound_facts.
+      inv_lstar.
+      inv_lstar.
+      bound_facts.
+      inv_lstar.
+      inv_lstar.
+      inv_lstar.
+      servers_done_contra.
+      inv_lstar.
+      bound_facts.
+      inv_lstar.
+      inv_lstar.
+      inv_lstar.
+      bound_facts.
+      inv_lstar.
+      inv_lstar.
+
+      (* Servers grabbed evidence *)
+      bound_facts.
+      inv_lstar.
+
+      
+      inv_lstar.
+      (* Servers grabbed the evidence *)
+      bound_facts.
+      inv_lstar.
+      inv_lstar.
+
+      (* aseq is peeled off on the server *)
+      inv_lstar.
+      inv_lstar.
+      
+      (* Main thread grabbed evidence again *)
+      inv_lstar.
+      inv_lstar.
+      servers_done_contra.
+      inv_lstar.
+      bound_facts.
+      inv_lstar.
+      inv_lstar.
+
+      (* Server grabbed evidence in correct sequence *)
+      inv_lstar.
+      bound_facts.
+      inv_lstar.
+      inv_lstar.
+      bound_facts.
+      inv_lstar.
+      inv_lstar.
+      inv_lstar.
+      bound_facts.
+      inv_lstar.
+      inv_lstar.
+      inv_lstar.
+
+      (* Server done processing request *)
+      inv_lstar.
+      admit.  (* Cannot be a Some event *)
+
+      (* Now execution must proceed on server *)
+      inv_lstar.
+      bound_facts.
+      inv_lstar.
+      inv_lstar.
+
+      (* Must now start processing t on Server 
+         ils (iconf (instr_compiler t) n0 e) (aResp ...) n *)
+      inv_lstar.
+      admit.  (* Cannot be Some e *)
+    
+      inv_lstar.
+      (* Entered ils on server for evaulating subterm *)
+      bound_facts.
+      inv_lstar.
+
+      assert (well_formed t).
+      {
+        admit.
+      }
+
+
+
+      edestruct at_world_decomp.
+      eassumption.
+      eassumption.
+      destruct_conjs.
+
+      assert (lstar (conf t n0 mt) x (stop n0 (aeval t n0 mt))).
+      {
+        eapply IHt.
+        eassumption.
+        eassumption.
+        eassumption.
+      }
+
+      subst.
+
+      admit. 
+    +
+      admit.
+      
+    +
+
+      
+      bound_facts.
+      inv_lstar.
+    +
+      inv_lstar.
+      bound_facts.
+      inv_lstar.
+
+      inv_lstar.
+      Focus 2.
+
+      inv_lstar.
+      bound_facts.
+      inv_lstar.
+      inv_lstar.
+
+      
+      inv_lstar.
+      inv_lstar.
+      
+      
+      
+
+      
+
+      
+
+      edestruct IHt.
+      eassumption.
+      admit.
+      admit.
+      
+
+      invc H0.
+      admit.
+
+      invc X.
+      inv_lstar.
+
+      invc H4.
+      unfold map_get in *.
+
+      break_if; try solve_by_inversion.
+      find_inversion.
+
+      unfold map_replace in *.
+      unfold map_remove in *.
+      rewrite Heqb in *.
+      unfold map_set in *.
+
+      assert (p4 = n0). admit.
+      subst. clear Heqb.
+
+      assert (
+
+      invc H10.
+     
+      
+      admit.
+    +
+      
+      
+
+
+
+    
+    inv_lstar.
+    inv_lstar.
+    inv_lstar.
+    admit.
+    bound_facts.
+    inv_lstar.
+
+    inv_lstar.
+    bound_facts.
+    inv_lstar.
+    inv_lstar.
+    admit.
+
+    bound_facts.
+    unfold wrap_server_config in *.
+    df.
+    inv_lstar.
+
+    unfold wrap_server_config in *.
+    df.
+    inv_lstar.
+    bound_facts.
+    inv_lstar.
+    inv_lstar.
+    inv_lstar.
+    inv_lstar.
+    inv_lstar.
+    inv_lstar.
+    inv_lstar.
+    inv_lstar.
+    servers_done_contra.
+    inv_lstar.
+    bound_facts.
+    inv_lstar.
+    inv_lstar.
+    bound_facts.
+    inv_lstar.
+    inv_lstar.
+    inv_lstar.
+    servers_done_contra.
+
+    inv_lstar.
+    bound_facts.
+    inv_lstar.
+    inv_lstar.
+    inv_lstar.
+    bound_facts.
+    inv_lstar.
+    inv_lstar.
+    bound_facts.
+    inv_lstar.
+    inv_lstar.
+    bound_facts.
+    inv_lstar.
+    inv_lstar.
+    inv_lstar.
+    inv_lstar.
+    inv_lstar.
+    inv_lstar
+    
+
+
+
+    
+    inv_lstar.
+    bound_facts.
+    inv_lstar.
+    inv_lstar.
+    inv_lstar.
+    inv_lstar.
+    inv_lstar.
+    servers_done_contra.
+    inv_lstar.
+    bound_facts.
+    inv_lstar.
+    inv_lstar.
+    bound_facts.
+    inv_lstar.
+    inv_lstar.
+    inv_lstar.
+    servers_done_contra.
+    inv_lstar.
+    bound_facts.
+    inv_lstar.
+    inv_lstar.
+    inv_lstar.
+    bound_facts.
+    inv_lstar.
+    inv_lstar.
+    bound_facts.
+    inv_lstar.
+    inv_lstar.
+    bound_facts.
+    inv_lstar.
+    inv_lstar.
+    inv_lstar.
+    inv_lstar.
+    inv_lstar.
+    inv_lstar.
+    servers_done_contra.
+    inv_lstar.
+    bound_facts.
+    inv_lstar.
+    inv_lstar.
+    inv_lstar.
+    bound_facts.
+    inv_lstar.
+    inv_lstar.
+    bound_facts.
+    inv_lstar.
+    inv_lstar.
+    inv_lstar.
+    bound_facts.
+    inv_lstar.
+    inv_lstar.
+    inv_lstar.
+    inv_lstar.
+    inv_lstar.
+    bound_facts.
+    inv_lstar.
+    inv_lstar.
+    inv_lstar.
+    bound_facts.
+    inv_lstar.
+    inv_lstar.
+    inv_lstar.
+    inv_lstar.
+    bound_facts.
+    inv_lstar.
+    invc H0.
+    invc X.
+    invc H9.
+    invc H2.
+    servers_done_contra.
+    invc X.
+    invc H9.
+    invc H0.
+    df.
+    bound_facts.
+    servers_done_contra.
+    df.
+    bound_facts.
+    inv_lstar.
+    df.
+    invc X.
+    inv_lstar.
+    df.
+    bound_facts.
+    invc H2.
+    servers_done_contra.
+    invc X.
+    solve_by_inversion.
+    df.
+    bound_facts.
+    invc H0.
+    unfold servers_done in *.
+    pose (H1 n0 i'0).
+    forward e2.
+    econstructor.
+    df.
+    try rewrite Nat.eqb_refl in *.
+    tauto.
+    concludes.
+    destruct_conjs.
+    subst. 
+    inv_lstar.
+    
+
+
+
+
+
+    
+
+    admit.
+
+    admit.
+
+    admit.
+
+    admit.
+
+    admit.
+
+    admit.
+
+    admit.
+
+
+    
+    HEREEEEEE
+    admit.
+*)
+  -
+    do_wf_pieces.
+
+    (*
+    assert (
+        exists (tr1: list Ev) e' servs_mid (h_mid:heap),
+          lstar_world
+           (worldTermC (iconf (instr_compiler t1) p e)
+              (combine (map_dom (copland_compliment_l t1 [])) (map wrap_server_config (copland_compliment_l t1 [])))) Empty tr1
+           (worldTermC (istop p e') servs_mid) h_mid /\
+          exists (tr2: list Ev) e'',
+            lstar_world
+           (worldTermC (iconf (instr_compiler t2) p e')
+              (combine (map_dom (copland_compliment_l t2 [])) (map wrap_server_config (copland_compliment_l t2 [])))) Empty (*h_mid*) tr2
+           (worldTermC (istop p e'') servs') h' /\
+            tr = tr1 ++ tr2).
+    {
+     *)
+    
+      
+
+
+    edestruct lstar_world_lseq_decomp.
+    eassumption.
+    eassumption.
+      
+    destruct_conjs.
+
+    subst.
+
+    
+
+    pose (IHt1 p e H4 Empty x H5 H2 H6).
+
+    pose (IHt2 p H4 e' h' H8 servs' H3 H9).
+    repeat concludes.
+
+    eapply lstar_silent_tran.
+    econstructor.
+
+    eapply lstar_transitive.
+    Check lstar_stls.
+    eapply lstar_stls.
+    eassumption.
+
+    eapply lstar_silent_tran.
+    apply stlseqstop.
+
+    eapply evshape_trace_irrel; eauto.
+    Defined.
+
+    
+    
+    
+    
+    
+
+
+  
+
+
+
+
+
+
+
+
+
+
+
+
+
+
+
+
+
+
+(*
+Lemma world_refines_lts_event_ordering:
+  forall t p e e' h h' tr et (wt:WorldTerm),
+    well_formed t ->
+   (* let wt := build_world_term t p e in (*(InstrSt*configs)*) *)
+    lstar_world (build_world_term t p e) h tr (donePlat p e') h' ->
+    LTS.lstar (conf t p et) tr (stop p (aeval t p et)).
+Proof.
+
+  
+  intros.
+  generalizeEverythingElse t.
+  induction t; intros.
+  -
+    destruct a.
+    +
+      df.
+      destruct r.
+      df.
+      invc H0.
+      ++
+        df.
+        invc H1.
+  
+Abort.
+*)
+
+
+
+
+HERE
+
+Inductive PlatSt: Set :=
+| stop: Plc -> Evidence -> St
+| conf: AnnoTerm -> Plc -> Evidence -> St
+| rem: nat -> Loc -> Plc -> St -> St
+| ls: St -> AnnoTerm -> St
+(*| bsl: nat -> St -> AnnoTerm -> Plc -> Evidence -> St
+| bsr: nat -> Evidence -> St -> St
+| bp: nat -> Loc -> Loc -> St -> St -> St*) .
+
+
+
+
+
+Record PlatformState : Type := mk_plat
+                         {plat_pl:Plc ;
+                          plat_trace:list Ev ;
+                          plat_store:heap}.
+
+Definition start (st:PlatformState) (places:(CVM unit) * setup) : PlatformState.
+Admitted.
+
+Definition run_it (me:Plc) (t:AnnoTerm) : PlatformState :=
+  start (mk_plat me [] []) (orchestrate t).
+
+Definition getLocs (t:Term) (m:MapC (Plc*Plc) (list Loc)): list Loc.
+Admitted.
+
+Definition fromSome{A:Type} (default:A) (opt:option A): A :=
+  match opt with
+  | Some x => x
+  | _ => default
+  end.
+
+Definition run_it_term (me:Plc) (t:Term) (m:MapC (Plc*Plc) (list Loc)) : PlatformState :=
+  let annt := snd (anno' t 0 (getLocs t m)) in
+  run_it me annt.
+
+
+
+
+
+
+
+
+
+
+
+(** * Transitive Closures *)
+
+Inductive lstar: InstrSt -> list Ev -> InstrSt -> Prop :=
+| lstar_refl: forall st, lstar st [] st
+| lstar_tran: forall st0 e st1 tr st2,
+    Instr_step st0 (Some e) st1 -> lstar st1 tr st2 -> lstar st0 (e :: tr) st2
+| lstar_silent_tran: forall st0 st1 tr st2,
+    Instr_step st0 None st1 -> lstar st1 tr st2 -> lstar st0 tr st2.
+Hint Resolve lstar_refl : core.
+
+Lemma lstar_transitive:
+  forall st0 tr0 st1 tr1 st2,
+    lstar st0 tr0 st1 ->
+    lstar st1 tr1 st2 ->
+    lstar st0 (tr0 ++ tr1) st2.
+Proof.
+  intros.
+  induction H.
+  - rewrite app_nil_l; auto.
+  - apply IHlstar in H0.
+    rewrite <- app_comm_cons.
+    eapply lstar_tran; eauto.
+  - apply IHlstar in H0.
+    eapply lstar_silent_tran; eauto.
+Qed.
+
+(** Transitive closure without labels. *)
+
+Inductive star: InstrSt -> InstrSt -> Prop :=
+| star_refl: forall st, star st st
+| star_tran: forall st0 e st1 st2,
+    Instr_step st0 e st1 -> star st1 st2 -> star st0 st2.
+Hint Resolve star_refl : core.
+
+Lemma star_transitive:
+  forall st0 st1 st2,
+    star st0 st1 ->
+    star st1 st2 ->
+    star st0 st2.
+Proof.
+  intros.
+  induction H; auto.
+  apply IHstar in H0.
+  eapply star_tran; eauto.
+Qed.
+
+Lemma lstar_star:
+  forall st0 tr st1,
+    lstar st0 tr st1 -> star st0 st1.
+Proof.
+  intros.
+  induction H; auto;
+    eapply star_tran; eauto.
+Qed.
+
+Lemma star_lstar:
+  forall st0 st1,
+    star st0 st1 -> exists tr, lstar st0 tr st1.
+Proof.
+  intros.
+  induction H; auto.
+  - exists []; auto.
+  - destruct IHstar as [tr G].
+    destruct e.
+    + exists (e :: tr).
+      eapply lstar_tran; eauto.
+    + exists tr.
+      eapply lstar_silent_tran; eauto.
+Qed.
+
+(*
+Lemma star_seval:
+  forall st0 st1,
+    star st0 st1 -> seval st0 = seval st1.
+Proof.
+  intros.
+  induction H; auto.
+  apply step_seval in H; auto.
+  rewrite H; auto.
+Qed.
+
+Lemma steps_preserves_eval:
+  forall t p p' e0 e1,
+    star (conf t p e0) (stop p' e1) ->
+    aeval t p e0 = e1.
+Proof.
+  intros.
+  apply star_seval in H.
+  simpl in H; auto.
+Qed.
+*)
+
+(** * Correct Path Exists *)
+
+(*
+Lemma star_strem:
+  forall st0 st1 j p loc,
+    star st0 st1 -> star (rem j loc p st0) (rem j loc p st1).
+Proof.
+  intros.
+  induction H; auto.
+  eapply star_tran; eauto.
+Qed.
+*)
+
+Lemma star_stls:
+  forall st0 st1 t,
+    star st0 st1 -> star (ils st0 t) (ils st1 t).
+Proof.
+  intros.
+  induction H; auto.
+  eapply star_tran; eauto.
+Qed.
+
+(*
+Lemma star_stbsl:
+  forall st0 st1 j t p e,
+    star st0 st1 ->
+    star (bsl j st0 t p e) (bsl j st1 t p e).
+Proof.
+  intros.
+  induction H; auto.
+  eapply star_tran; eauto.
+Qed.
+
+Lemma star_stbsr:
+  forall st0 st1 j e,
+    star st0 st1 ->
+    star (bsr j e st0) (bsr j e st1).
+Proof.
+  intros.
+  induction H; auto.
+  eapply star_tran; eauto.
+Qed.
+*)
+
+(* Congruence lemmas for Copland LTS semantics *)
+Lemma lstar_stls :
+  forall st0 st1 t tr,
+    lstar st0 tr st1 -> lstar (ils st0 t) tr (ils st1 t).
+Proof.
+  intros.
+  induction H; auto.
+  eapply lstar_tran; eauto.
+  eapply lstar_silent_tran; eauto.
+Qed.
+
+(*
+Lemma lstar_strem : forall st st' tr p r loc,
+    lstar st tr
+          st' ->
+    lstar (rem r loc p st) tr (rem r loc p st').
+Proof.
+  intros.
+  induction H; auto.
+  eapply lstar_tran; eauto.
+  eapply lstar_silent_tran; eauto.
+Defined.
+*)
+
+(*
+Lemma lstar_stbsl:
+  forall st0 st1 j t p e tr,
+    lstar st0 tr st1 ->
+    lstar (bsl j st0 t p e) tr (bsl j st1 t p e).
+Proof.
+  intros.
+  induction H; auto.
+  eapply lstar_tran; eauto.
+  eapply lstar_silent_tran; eauto.
+Defined.
+
+Lemma lstar_stbsr:
+  forall st0 st1 j e tr,
+    lstar st0 tr st1 ->
+    lstar (bsr j e st0) tr (bsr j e st1).
+Proof.
+  intros.
+  induction H; auto.
+  eapply lstar_tran; eauto.
+  eapply lstar_silent_tran; eauto.
+Defined.
+
+Lemma star_stbp:
+  forall st0 st1 st2 st3 j xi yi,
+    star st0 st1 ->
+    star st2 st3 ->
+    star (bp j xi yi st0 st2) (bp j xi yi st1 st3).
+Proof.
+  intros.
+  induction H; auto.
+  - induction H0; auto.
+    eapply star_tran; eauto.
+  - eapply star_tran; eauto.
+Qed.
+ *)
+
+
+(*
+Inductive InstrSt: Set :=
+| istop: cvm_st -> InstrSt
+| iconf: AnnoInstr -> cvm_st -> InstrSt
+(*| rem: nat -> Loc -> Plc -> St -> St *)
+| ils: InstrSt -> AnnoInstr -> InstrSt
+(*| bsl: nat -> St -> AnnoTerm -> Plc -> Evidence -> St
+| bsr: nat -> Evidence -> St -> St
+| bp: nat -> Loc -> Loc -> St -> St -> St*) .
+*)
+
+(*
+Theorem correct_path_exists:
+  forall p e i,
+    exists st',
+    star (iconf i p e) (istop p st').
+Proof.
+  induction i; intros; simpl; eauto.
+  -
+    eexists.
+
+    eapply star_tran; eauto.
+    (*
+  - destruct p.
+    eapply star_tran; eauto.
+    eapply star_transitive.
+    apply star_strem.
+    apply IHt.
+    eapply star_tran; eauto. *)
+  -
+    edestruct IHi1.
+    edestruct IHi2.
+    eexists.
+    eapply star_tran.
+    econstructor.
+    eapply star_transitive.
+    apply star_stls.
+    eassumption.
+    eapply star_tran.
+    apply seqStop.
+    Abort.
+
+    (*
+    
+  - eapply star_tran; eauto.
+    eapply star_transitive.
+    apply star_stbsl.
+    apply IHt1.
+    eapply star_tran; eauto.
+    eapply star_transitive.
+    apply star_stbsr.
+    apply IHt2.
+    eapply star_tran; eauto.
+  -
+    repeat dest_range.
+    (*destruct p; destruct p0. *)
+    eapply star_tran; eauto.
+    eapply star_transitive.
+    apply star_stbp.
+    apply IHt1.
+    apply IHt2.
+    eapply star_tran; eauto.
+Qed.
+*)
+*)
+
+(** * Progress *)
+
+Definition halt st :=
+  match st with
+  | istop _ _ _ => True
+  | _ => False
+  end.
+
+(*
+(** The Instr_step relation nevers gets stuck. *)
+
+Theorem never_stuck:
+  forall st0,
+    halt st0 \/ exists e st1, Instr_step st0 e st1.
+Proof.
+  induction st0.
+  - left; simpl; auto.
+    
+  - right.
+    destruct a.
+    + exists (Some (tr_asp_instr n0 n p)).
+      eapply ex_intro; eauto.
+
+      (*
+    + exists (Some (req (fst r) (fst p) n n0 (unanno a))).
+      repeat dest_range.
+      eapply ex_intro; eauto. *)
+    + exists None.
+      eapply ex_intro; eauto.
+      (*
+      
+    + exists (Some (split (fst r) n)).
+      eapply ex_intro; eauto.
+      
+    + exists (Some (splitp (fst r) (fst p) (*(fst p0)*) n)).
+      (*destruct p; destruct p0. *)
+      repeat dest_range.
+      eapply ex_intro; eauto. *)
+     
+    (*
+  - right.
+    destruct IHst0.
+    + destruct st0; simpl in H; try tauto.
+      exists (Some (rpy (pred n) n0 n1 n2)).
+      eapply ex_intro; eauto.
+    + destruct H as [e H].
+      exists e.
+      destruct H as [st1 H].
+      exists (rem n n0 n1 st1). auto. *)
+  - right.
+    destruct IHst0.
+    + destruct st0; simpl in H; try tauto.
+      exists None. eapply ex_intro; eauto.
+    + destruct H as [e H].
+      exists e.
+      destruct H as [st H].
+      exists (ils st a). auto.
+      (*
+      
+  - right.
+    destruct IHst0.
+    + destruct st0; simpl in H; try tauto.
+      exists None. eapply ex_intro; eauto.
+    + destruct H as [e0 H].
+      exists e0.
+      destruct H as [st H].
+      exists (bsl n st a n0 e). auto.
+  - right.
+    destruct IHst0.
+    + destruct st0; simpl in H; try tauto.
+      exists (Some (join (pred n) n0)).
+      eapply ex_intro; eauto.
+    + destruct H as [e0 H].
+      exists e0.
+      destruct H as [st H].
+      exists (bsr n e st). auto.
+      
+  - right.
+    destruct IHst0_1 as [H|H].
+    + destruct st0_1; simpl in H; try tauto.
+      clear H.
+      destruct IHst0_2.
+      * destruct st0_2; simpl in H; try tauto.
+        exists (Some (joinp (pred n) n0 n1 n3)).
+        eapply ex_intro; eauto.
+      * destruct H as [e0 H].
+        exists e0.
+        destruct H as [st H].
+        exists (bp n n0 n1 (stop n2 e) st). auto.
+    + destruct H as [e0 H].
+      exists e0.
+      destruct H as [st H].
+      exists (bp n n0 n1 st st0_2). auto.
+*)
+Qed.
+*)
+
+(** * Termination *)
+
+Inductive nstar: nat -> InstrSt -> InstrSt -> Prop :=
+| nstar_refl: forall st, nstar 0 st st
+| nstar_tran: forall st0 st1 st2 e n,
+    nstar n st0 st1 -> Instr_step st1 e st2 -> nstar (S n) st0 st2.
+Hint Resolve nstar_refl : core.
+
+Require Import PeanoNat.
+
+Lemma nstar_transitive:
+  forall m n st0 st1 st2,
+    nstar m st0 st1 ->
+    nstar n st1 st2 ->
+    nstar (m + n) st0 st2.
+Proof.
+  intros.
+  induction H0.
+  rewrite Nat.add_0_r; auto.
+  apply IHnstar in H.
+  eapply nstar_tran in H; eauto.
+  rewrite plus_n_Sm in H.
+  eauto.
+Qed.
+
+Lemma nstar_star:
+  forall n st0 st1,
+    nstar n st0 st1 -> star st0 st1.
+Proof.
+  intros.
+  induction H; auto.
+  eapply star_transitive; eauto.
+  eapply star_tran; eauto.
+Qed.
+
+Lemma star_nstar:
+  forall st0 st1,
+    star st0 st1 ->
+    exists n, nstar n st0 st1.
+Proof.
+  intros.
+  induction H.
+  - exists 0; auto.
+  - destruct IHstar as [n G].
+    exists (S n).
+    rewrite <- Nat.add_1_l.
+    eapply nstar_transitive; eauto.
+    eapply nstar_tran; eauto.
+Qed.
+
+
+(*
+
+(** Size of a term (number of steps to reduce). *)
+
+Fixpoint tsize t: nat :=
+  match t with
+  | aprimInstr _ _ => 1
+  (*| aatt _ _ _ _ x => 2 + tsize x *)
+  | aseq x y => 2 + tsize x + tsize y
+  (*| abseq _ _ _ x y => 3 + tsize x + tsize y
+  | abpar _ _ _ _ x y => 2 + tsize x + tsize y *)
+  end.
+
+(** Size of a state (number of steps to reduce). *)
+
+Fixpoint ssize s: nat :=
+  match s with
+  | istop _ _ => 0
+  | iconf t _ _ => tsize t
+  (*| rem _ _ _ x => 1 + ssize x *)
+  | ils x t => 1 + ssize x + tsize t
+  (*| bsl _ x t _ _ => 2 + ssize x + tsize t
+  | bsr _ _ x => 1 + ssize x
+  | bp _ _ _ x y => 1 + ssize x + ssize y *)
+  end.
+
+(** Halt state has size 0. *)
+
+Lemma halt_size:
+  forall st,
+    halt st <-> ssize st = 0.
+Proof.
+  split; intros.
+  - destruct st; simpl in H; try tauto.
+  - destruct st; simpl in H; try tauto;
+      try discriminate.
+    + simpl; auto.
+    + destruct a; simpl in H; discriminate.
+Qed.
+
+Require Import Lia.
+(** A state decreases its size by one. *)
+
+Lemma step_size:
+  forall st0 e st1,
+    Instr_step st0 e st1 ->
+    S (ssize st1) = ssize st0.
+Proof.
+  intros.
+  induction H; simpl; auto; lia.
+Qed.
+
+Lemma step_count:
+  forall n t p e st,
+    nstar n (iconf t p e) st ->
+    tsize t = n + ssize st.
+Proof.
+  induction n; intros.
+  - inv H; simpl; auto.
+  - inv H.
+    apply IHn in H1.
+    rewrite H1.
+    apply step_size in H2.
+    lia.
+Qed.
+
+(** Every run terminates. *)
+
+Theorem steps_to_stop:
+  forall t p e st,
+    nstar (tsize t) (iconf t p e) st ->
+    halt st.
+Proof.
+  intros.
+  apply step_count in H.
+  apply halt_size.
+  lia.
+Qed.
+
+(** * Numbered Labeled Transitions *)
+
+Inductive nlstar: nat -> InstrSt -> list Ev -> InstrSt -> Prop :=
+| nlstar_refl: forall st, nlstar 0 st [] st
+| nlstar_tran: forall n st0 e st1 tr st2,
+    Instr_step st0 (Some e) st1 -> nlstar n st1 tr st2 -> nlstar (S n) st0 (e :: tr) st2
+| nlstar_silent_tran: forall n st0 st1 tr st2,
+    Instr_step st0 None st1 -> nlstar n st1 tr st2 -> nlstar (S n) st0 tr st2.
+Hint Resolve nlstar_refl : core.
+
+Lemma nlstar_transitive:
+  forall m n st0 tr0 st1 tr1 st2,
+    nlstar m st0 tr0 st1 ->
+    nlstar n st1 tr1 st2 ->
+    nlstar (m + n) st0 (tr0 ++ tr1) st2.
+Proof.
+  intros.
+  induction H.
+  - rewrite app_nil_l; auto.
+  - apply IHnlstar in H0.
+    rewrite <- app_comm_cons.
+    eapply nlstar_tran; eauto.
+  - apply IHnlstar in H0.
+    eapply nlstar_silent_tran; eauto.
+Qed.
+
+Lemma nlstar_lstar:
+  forall n st0 tr st1,
+    nlstar n st0 tr st1 -> lstar st0 tr st1.
+Proof.
+  intros.
+  induction H; auto.
+  - eapply lstar_tran; eauto.
+  - eapply lstar_silent_tran; eauto.
+Qed.
+
+Lemma lstar_nlstar:
+  forall st0 tr st1,
+    lstar st0 tr st1 ->
+    exists n, nlstar n st0 tr st1.
+Proof.
+  intros.
+  induction H.
+  - exists 0; auto.
+  - destruct IHlstar as [n G].
+    exists (S n).
+    eapply nlstar_tran; eauto.
+  - destruct IHlstar as [n G].
+    exists (S n).
+    eapply nlstar_silent_tran; eauto.
+Qed.
+
+Lemma nlstar_step_size:
+  forall n st0 tr st1,
+    nlstar n st0 tr st1 ->
+    ssize st1 <= ssize st0.
+Proof.
+  intros.
+  induction H; auto;
+    apply step_size in H;
+    lia.
+Qed.
+
+Require Import Minus.
+
+Lemma lstar_nlstar_size:
+  forall st0 tr st1,
+    lstar st0 tr st1 ->
+    nlstar (ssize st0 - ssize st1) st0 tr st1.
+Proof.
+  intros.
+  induction H.
+  - rewrite Nat.sub_diag; auto.
+  - pose proof H as G.
+    apply step_size in G.
+    rewrite <- G.
+    rewrite <- minus_Sn_m.
+    + eapply nlstar_tran; eauto.
+    + apply nlstar_step_size in IHlstar; auto.
+  - pose proof H as G.
+    apply step_size in G.
+    rewrite <- G.
+    rewrite <- minus_Sn_m.
+    + eapply nlstar_silent_tran; eauto.
+    + apply nlstar_step_size in IHlstar; auto.
+Qed.
+
+(** The reverse version of [nlstar]. *)
+
+Inductive rlstar: nat -> InstrSt -> list Ev -> InstrSt -> Prop :=
+| rlstar_refl: forall st, rlstar 0 st [] st
+| rlstar_tran: forall n st0 e st1 tr st2,
+    rlstar n st0 tr st1 -> Instr_step st1 (Some e) st2 ->
+    rlstar (S n) st0 (tr ++ [e]) st2
+| rlstar_silent_tran: forall n st0 st1 tr st2,
+    rlstar n st0 tr st1 -> Instr_step st1 None st2 ->
+    rlstar (S n) st0 tr st2.
+Hint Resolve rlstar_refl : core.
+
+Lemma rlstar_transitive:
+  forall m n st0 tr0 st1 tr1 st2,
+    rlstar m st0 tr0 st1 ->
+    rlstar n st1 tr1 st2 ->
+    rlstar (m + n) st0 (tr0 ++ tr1) st2.
+Proof.
+  intros.
+  induction H0.
+  - rewrite Nat.add_0_r; rewrite app_nil_r; simpl; auto.
+  - apply IHrlstar in H.
+    rewrite Nat.add_succ_r.
+    rewrite app_assoc.
+    eapply rlstar_tran; eauto.
+  - apply IHrlstar in H.
+    rewrite Nat.add_succ_r.
+    eapply rlstar_silent_tran; eauto.
+Qed.
+
+Lemma rlstar_lstar:
+  forall n st0 tr st1,
+    rlstar n st0 tr st1 -> lstar st0 tr st1.
+Proof.
+  intros.
+  induction H; auto.
+  - eapply lstar_transitive; eauto.
+    eapply lstar_tran; eauto.
+  - rewrite <- app_nil_r with (l:=tr).
+    eapply lstar_transitive; eauto.
+    apply lstar_silent_tran with st2; auto.
+Qed.
+
+Lemma lstar_rlstar:
+  forall st0 tr st1,
+    lstar st0 tr st1 ->
+    exists n, rlstar n st0 tr st1.
+Proof.
+  intros.
+  induction H.
+  - exists 0; auto.
+  - destruct IHlstar as [n G].
+    exists (S n).
+    cut (rlstar (1 + n) st0 ([e] ++ tr) st2).
+    simpl; auto.
+    eapply rlstar_transitive; eauto.
+    cut (rlstar 1 st0 ([] ++ [e]) st1).
+    simpl; auto.
+    eapply rlstar_tran; eauto.
+  - destruct IHlstar as [n G].
+    exists (S n).
+    cut (rlstar (1 + n) st0 ([] ++ tr) st2).
+    rewrite app_nil_l; auto.
+    eapply rlstar_transitive; eauto.
+    eapply rlstar_silent_tran; eauto.
+Qed.
+
+Lemma rlstar_nlstar:
+  forall n st0 tr st1,
+    rlstar n st0 tr st1 <-> nlstar n st0 tr st1.
+Proof.
+  split; intros.
+  - induction H; auto.
+    + rewrite <- Nat.add_1_r.
+      eapply nlstar_transitive; eauto.
+      eapply nlstar_tran; eauto.
+    + rewrite <- Nat.add_1_r.
+      rewrite <- app_nil_r with (l:=tr).
+      eapply nlstar_transitive; eauto.
+      eapply nlstar_silent_tran; eauto.
+  - induction H; auto.
+    + rewrite <- Nat.add_1_l.
+      assert (G: e :: tr = [e] ++ tr).
+      simpl; auto.
+      rewrite G.
+      eapply rlstar_transitive; eauto.
+      rewrite <- app_nil_l with (l:=[e]).
+      eapply rlstar_tran; eauto.
+    + rewrite <- Nat.add_1_l.
+      rewrite <- app_nil_l with (l:=tr).
+      eapply rlstar_transitive; eauto.
+      eapply rlstar_silent_tran in H; eauto.
+Qed.
+
+ *)
+
+
+
+
+
+
+
+
+
+
+
+
+
+
+
+
+
+(* EXTRA 
+
+Lemma advance_servers_determ: forall ai m m' m'',
+    advance_servers ai m m' ->
+    advance_servers ai m m'' ->
+    m' = m''.
+Proof.
+Admitted.
+
+Lemma advance_ist_iff: forall x m m' p e,
+    advance_servers x m m' ->
+    advance_servers_ist (iconf x p e) m m'.
+Proof.
+Admitted.
+
+Lemma compliment_alseq_skip: forall r l t1 t2 m m',
+    (*well_formed (alseq r l t1 t2) -> *)
+    ws_instr (instr_compiler (alseq r l t1 t2)) m ->
+    advance_servers (instr_compiler t1) m m' ->
+    ws_instr (instr_compiler t1) m /\
+    ws_instr (instr_compiler t2) m'.
+Proof.
+  intros.
+  invc H.
+  split.
+  -
+    eassumption.
+  -
+    assert (m' = m'0).
+    {
+      eapply advance_servers_determ; eauto.
+    }
+    subst.
+    eauto.
+Defined.
+
+Lemma compliment_alseq_skip': forall r l t1 t2 m m',
+    (*well_formed (alseq r l t1 t2) -> *)
+    ws_instr (instr_compiler t1) m ->
+    advance_servers (instr_compiler t1) m m' ->
+    ws_instr (instr_compiler t2) m' ->
+    ws_instr (instr_compiler (alseq r l t1 t2)) m.  
+Proof.
+Admitted.
+
+
+Require Import Auto.
+
+Lemma compliment_focus: forall t1 t2,
+    ws_instr (instr_compiler t1) (copland_compliment t2 (copland_compliment t1 [])).
+Proof.
+Admitted.
+
+Lemma advance_assoc: forall t1 t2 m,
+    advance_servers (instr_compiler t1) (copland_compliment t2 (copland_compliment t1 m))
+                    (copland_compliment t2 m).
+Proof.
+Admitted.
+
+
+(*
+Fixpoint num_server_req_handles (ai:AnnoInstr) (toPl:Plc) : nat :=
+  match ai with
+  | aprimInstr i pi => 0
+  | aReq _ _ _ _ _ (pl,_) => if (toPl =? pl) then 1 else 0
+  | aseq ai1 ai2 =>
+    (num_server_req_handles ai1 toPl) +
+    (num_server_req_handles ai2 toPl)
+  end.
+
+Fixpoint num_server_req_handles_ist (iSt:InstrSt) (toPl:Plc) : nat :=
+  match iSt with
+  | istop _ _ => 0
+  | iconf ai _ _ => (num_server_req_handles ai toPl)
+  | iWaitReq _ _ ai => (num_server_req_handles ai toPl)
+  | iDoRem iSt' _ => (num_server_req_handles_ist iSt' toPl)
+  | iSeqReqWaits iSt1 iSt2 =>
+    (num_server_req_handles_ist iSt1 toPl) +
+    (num_server_req_handles_ist iSt2 toPl)
+  | irpyWait _ _ _ _ => 0
+  | ils iSt ai =>
+    (num_server_req_handles_ist iSt toPl) +
+    (num_server_req_handles ai toPl)
+  end.
+
+(* 
+   Relates an AnnoInstr + its servers before executing 
+   that AnnoInstr, to its servers after.
+
+   Need to map over all instances of (aReq _ _ _ _ toPl) instructions in 
+   the client AnnoInstr and skip an iWaitReq at toPl for each. 
+
+   TODO:  use something like num_server_req_handles above to determine a 
+   predictable number of new "iWaitReq" instrSts to peel off front of each server st code 
+*)
+Definition advance_servers :
+  AnnoInstr ->
+  MapC Plc InstrSt ->
+  MapC Plc InstrSt -> Prop.
+Admitted.
+
+(* same as advance_servers, but for InstrSt *)
+Definition advance_servers_ist :
+  InstrSt ->
+  MapC Plc InstrSt ->
+  MapC Plc InstrSt -> Prop.
+Admitted.
+*)
+
+*)
