src/Place_Facts.v
@@ -1,0 +1,308 @@
+Require Import Maps Term_Defs StructTactics.
+
+Require Import List.
+Import ListNotations.
+
+(*
+Definition inc_vm_id (m:VMID_Map) (p:Plc) : (VM_ID*VMID_Map) :=
+  let val := map_get m p in
+  match val with
+  | Some v => (v,map_replace m p (v + 1))
+  | None => (0,map_set m p 1)
+  end.
+ *)
+
+Definition VMID_Map := (MapC VM_ID Plc).
+
+Fixpoint flatten_places' (t:Term) (n:nat) (m:MapC VM_ID Plc): (nat*(MapC VM_ID Plc)) :=
+  match t with
+  | asp a => (n,m)     
+  | att q t' =>
+    flatten_places' t' (n+1) (map_set m n q)              
+  | lseq t1 t2 =>
+    let '(n',m') := flatten_places' t1 n m in
+    flatten_places' t2 n' m'
+  end.
+
+Definition flatten_places (t:Term) : (MapC Plc VM_ID) :=
+  snd (flatten_places' t 1 []).
+
+
+
+(* TODO: import and use option monad scope/notation *)
+Fixpoint flatten_term (t:Term) (m:MapC Plc VM_ID): option Term :=
+  match t with
+  | asp a => Some (asp a)
+                
+  | att q t' =>
+    let mp := map_get m q in
+    let mt' := flatten_term t' m in
+    match (mp, mt') with
+    | (Some v, Some newTerm) => Some (att v newTerm)
+    | _ => None
+    end              
+  | lseq t1 t2 =>
+    let mt1 := flatten_term t1 m in
+    let mt2 := flatten_term t2 m in
+    match (mt1,mt2) with
+    | (Some new_t1, Some new_t2) => Some (lseq new_t1 new_t2)
+    | _ => None
+    end
+end.
+
+Fixpoint term_places' (t:Term) (ls:list Plc): list Plc :=
+  match t with
+  | asp _ => ls   
+  | att q t' =>
+    term_places' t' (q::ls)              
+  | lseq t1 t2 =>
+    term_places' t2 (term_places' t1 ls)
+  end.
+
+Definition term_places (t:Term): list Plc :=
+  term_places' t [].
+
+Require Import Auto.
+
+Inductive term_places_r : Term -> Plc -> Prop :=
+| atPlace: forall q t', term_places_r (att q t') q
+| atRecPlace: forall x q t',
+    term_places_r t' x ->
+    term_places_r (att q t') x
+| atLseqPlacel: forall t1 t2 p,
+    term_places_r t1 p ->
+    term_places_r (lseq t1 t2) p
+| atLseqPlacer: forall t1 t2 p,
+    term_places_r t2 p ->
+    term_places_r (lseq t1 t2) p.
+
+Set Nested Proofs Allowed.
+Require Import Coq.Arith.PeanoNat.
+
+Lemma term_places'_cumul: forall t p ls,
+    In p ls ->
+    In p (term_places' t ls).
+Proof.
+  induction t; intros.
+  -
+    df.
+    eassumption.
+  -
+    df.
+    assert (In p (term_places' t (n::ls))).
+    {
+    eapply IHt.
+    right.
+    eassumption.
+    }
+    eassumption.
+  -
+    df.
+    eauto.
+Defined.
+
+Lemma places_input_order: forall t p n n0 ls,
+    In p (term_places' t (n :: n0 :: ls)) ->
+    In p (term_places' t (n0 :: n:: ls)).
+Proof.
+  intros.
+
+  assert (In p (n :: n0 :: ls) \/ In p (term_places' t [])).
+  {
+    admit.
+  }
+  destruct H0.
+  eapply term_places'_cumul.
+  admit.
+Admitted.
+
+Lemma lseq_places_fact: forall t1 t2 p ls,
+    In p (term_places' t2 (term_places' t1 ls)) ->
+    In p (term_places' t1 ls) \/ In p (term_places' t2 []).
+Proof.
+Admitted.
+
+Lemma lseq_places_assoc: forall t1 t2 p n ls,
+    In p (term_places' t2 (term_places' t1 (n :: ls))) ->
+    In p (term_places' t2 (n :: term_places' t1 ls)).
+Proof.
+Admitted.
+
+
+Lemma peel_one: forall t n ls p,
+    In p (term_places' t (n :: ls)) ->
+    p <> n ->
+    In p (term_places' t ls).
+Proof.
+  intros.
+  generalizeEverythingElse t.
+  induction t; intros.
+  -
+    df.
+    destruct H; try eauto.
+    congruence.
+  -
+    df.
+    eapply IHt.
+    Focus 2.
+    eassumption.
+    eapply places_input_order; eauto.
+  -
+    df.
+    assert (In p (term_places' t1 (n::ls)) \/ In p (term_places' t2 [])).
+    {
+      eapply lseq_places_fact; eauto.
+    }
+    destruct H1.
+    +
+      eapply term_places'_cumul.
+      eauto.
+    +
+      eapply IHt2 with (n:=n).
+      eapply lseq_places_assoc; eauto.
+      eassumption.
+Defined.
+
+(*
+Lemma fff: forall p t n,
+    In p (term_places' t []) ->
+    p <> n ->
+    In p (term_places' t [n]).
+Proof.
+Admitted.
+*)
+
+Lemma term_places_weaken: forall t p ls,
+    In p (term_places' t []) ->
+    In p (term_places' t ls).
+Proof.
+  intros.
+  generalizeEverythingElse t.
+  induction t; intros.
+  -
+    solve_by_inversion.
+  -
+    cbn in H.
+    destruct (Nat.eq_dec p n).
+    +
+      subst.
+      df.
+      eapply term_places'_cumul.
+      econstructor.
+      tauto.
+    +
+      assert (In p (term_places' t [])).
+      {
+        eapply peel_one; eauto.
+        (*
+        
+        
+        edestruct singleton_places_fact.
+        eassumption.
+        invc H0.
+        congruence.
+        invc H1.
+        eassumption. *)
+      }
+      df.
+      eauto.
+  -
+    df.
+    edestruct lseq_places_fact.
+    eassumption.
+    assert (In p (term_places' t1 ls)) by eauto.
+    eapply term_places'_cumul.
+    eassumption.
+    eauto.
+Defined.
+
+Lemma term_places_iff_rel: forall t p,
+    term_places_r t p <-> In p (term_places t).
+Proof.
+  split.
+  -
+    unfold term_places.
+    induction t; intros; df.
+    +
+      solve_by_inversion.
+    +
+      invc H.
+      ++
+        eapply term_places'_cumul; eauto.
+        econstructor.
+        tauto.
+      ++
+        concludes.
+
+        eapply term_places_weaken; eauto.
+    +
+      invc H.
+      ++
+        concludes.
+        eapply term_places'_cumul; eauto.
+      ++
+        concludes.
+        eapply term_places_weaken.
+        eassumption.
+  -
+    intros.
+    unfold term_places in *.
+    generalizeEverythingElse t.
+    induction t; intros; df.
+    +
+      solve_by_inversion.
+    +
+      destruct (Nat.eq_dec p n).
+      ++
+        subst.
+        econstructor.
+      ++
+        econstructor.
+        eapply IHt.
+        eapply peel_one; eauto.
+
+        (*
+
+        edestruct singleton_places_fact.
+        eassumption.
+        invc H0.
+        congruence.
+        invc H1.
+        eassumption. *)
+    +
+      assert (In p (term_places' t1 []) \/ In p (term_places' t2 [])).
+      {       
+        eapply lseq_places_fact; eauto.
+      }
+      destruct H0.
+      ++
+        econstructor; eauto.
+      ++
+        apply atLseqPlacer.
+        eauto.
+Defined.
+
+(*
+Definition flatten_places (t:Term) : (MapC Plc VM_ID) :=
+  snd (flatten_places' t 1 []).
+ *)
+
+Lemma places_match: forall t,
+    map_dom (flatten_places t) = term_places t.
+Proof.
+Admitted.
+
+
+Lemma flatten_some: forall t,
+  (*term_places_r t p ->
+  In p (map_dom m) -> *)
+  (*map_dom m = term_places t -> *)
+  exists t', flatten_term t (flatten_places t) = Some t'.
+Proof.
+Admitted.
+
+Definition t1 := att 1 (asp (ASPC 1 [])).
+Definition t2 := (asp (ASPC 2 [])).
+Definition myterm := att 1 (lseq t1 (att 2 (lseq t2 (att 3 t1)))).
+
+Compute flatten_places myterm.
